FormalSystems/Chomsky/Regular/RegularGrammar.lean
@@ -1,8 +1,24 @@
-import FormalSystems.Chomsky.ContextFree.ContextFreeGrammar
-
 import Mathlib.Data.Finset.Basic
 import Mathlib.Data.Prod.Lex
 
+import FormalSystems.Chomsky.ContextFree.ContextFreeGrammar
+--================================================================================
+-- File: RegularGrammar
+/-  Containts Regular production definition and regular derivation
+    definition, as well as muliple coercions, e.g. to
+    context-free derivations.
+-/
+--================================================================================
+
+/--Inductive structure: A regular production has one of three shapes:
+
+  - `V → ε`,
+
+  - `V → Z` or
+
+  - `V → Z × V`,
+
+  where V is the finset of variable/non-terminal and Z of terminal symbols.-/
 inductive RegularProduction (Z: Finset α) (V: Finset nt) where
   /--`V → ε`-/
   | eps (lhs: V)
@@ -12,26 +28,33 @@ inductive RegularProduction (Z: Finset α) (V: Finset nt) where
   | cons (lhs: V) (rhs: Z × V)
   deriving DecidableEq
 
+/--A regular productions left-hand side.-/
 def RegularProduction.lhs : RegularProduction Z V → V
   | eps l => l
   | alpha l _ => l
   | cons l _ => l
 
+/--A regular productions right-hand side.-/
 def RegularProduction.rhs : RegularProduction Z V → Word (V ⊕ Z)
   | eps _ => ε
   | alpha _ a => [.inr a]
   | cons _ ⟨ a, A ⟩ => [.inr a, .inl A]
 
+/--The proposition that captures whether a regular production
+  goes to ε.-/
 def RegularProduction.isEps : RegularProduction Z V → Prop
   | eps _ => True
   | _ => False
 
+/--Get the regular productions right-hand side, but as a tuple
+  over Z and V.-/
 def RegularProduction.getRhs (p: RegularProduction Z V) : Option Z × Option V :=
   match p with
   | cons _ ⟨a, X⟩ => (.some a, .some X)
   | alpha _ a => (.some a, .none)
   | eps _ => (.none, .none)
 
+/--Prove that .isEps is a decidable predicate.-/
 instance { α nt: Type } { Z: Finset α } { V: Finset nt } :
   DecidablePred (@RegularProduction.isEps α Z nt V) := fun x =>
   match x with
@@ -39,12 +62,14 @@ instance { α nt: Type } { Z: Finset α } { V: Finset nt } :
   | RegularProduction.alpha _ _ => Decidable.isFalse (λh => h)
   | RegularProduction.cons _ _ => Decidable.isFalse (λh => h)
 
+/--Coerve regular productions in context-free productions.-/
 instance : Coe (RegularProduction Z V) (ContextFreeProduction Z V) where
   coe p := {
     lhs := p.lhs,
     rhs := p.rhs,
   }
 
+/--Embed regular productions in context-free productions.-/
 def RegularProduction.toContextFree : RegularProduction Z V ↪ ContextFreeProduction Z V where
   toFun := Coe.coe
   inj' p₁ p₂ := by
@@ -67,27 +92,35 @@ def RegularProduction.toContextFree : RegularProduction Z V ↪ ContextFreeProdu
         rw [List.cons_eq_cons] at hr; simp at hr
         simp [hl, hr]
 
+/--Coerce regular productions in generic productions.-/
 def RegularProduction.toProduction : RegularProduction Z V ↪ GenericProduction Z V :=
   toContextFree.trans ContextFreeProduction.toProduction
 
+/--Regular productions are instances of generic productions.-/
 instance : Production α nt RegularProduction :=
   Production.fromEmbedding $ fun _ _ => RegularProduction.toProduction
 
+/--Regular productions are instances of context-free productions.-/
 instance : Production.ContextFree α nt RegularProduction where
   lhs_var p := p.lhs
   lhs_eq_lhs _ := by rfl
 
+/--Theorem: .getRhs acts as expected with regard to .rhs-/
 theorem RegularProduction.rhs_eq_deconstr_rhs (p: RegularProduction Z V):
   Production.rhs p =
     Word.mk (Sum.inr <$> p.getRhs.1.toList) *
     Word.mk (Sum.inl <$> p.getRhs.2.toList) := by
   cases p <;> rfl
 
+/--Theorem: .lhs acts as expected.-/
 theorem RegularProduction.lhs_eq_production_lhs { p: RegularProduction Z V }:
   Production.lhs p = [.inl p.lhs] := by rfl
 
+/--A regular grammar is an instance of a grammar, where the set of productions
+  is reduced to those, that are regular.-/
 def RegularGrammar (α nt: Type) := @Grammar α nt RegularProduction _
 
+/--Coerce regular grammars in generic grammars.-/
 instance : Coe (RegularGrammar α nt) (@Grammar α nt GenericProduction _) where
   coe g := { g with
     productions := g.productions.map RegularProduction.toProduction
@@ -97,14 +130,18 @@ variable { G: RegularGrammar α nt } { p: G.productions }
 
 open Grammar
 
+/--Theorem: The result of`V→ε`regular productions is`ε`.-/
 theorem RegularProduction.eps_step_result:
   p.val = RegularProduction.eps v → (DerivationStep.fromRule p).result = ε := by
   intro h; simp [DerivationStep.fromRule, DerivationStep.result, h]; rfl
 
+/--Theorem: The result of`V→v*z`regular productions is`v*z`.-/
 theorem RegularProduction.cons_step_result:
   p.val = .cons v (w, b) → (DerivationStep.fromRule p).result = [.inr w, .inl b] := by
   intro h; simp [DerivationStep.fromRule, DerivationStep.result, h]; rfl
 
+/--Theorem: .isEps is true implies we have a regular production
+  constructed with the .eps constructor.-/
 theorem RegularProduction.eq_eps_from_isEps
   { Z: Finset α } { V: Finset nt }
   { p: RegularProduction Z V }:
@@ -115,6 +152,36 @@ theorem RegularProduction.eq_eps_from_isEps
 
 namespace RegularGrammar
 
+/--Inductive structure: Regular Derivations in G from variables v to
+  (fully terminal) words w are constructed using three possible constructors.
+  Note: This is defined in such a way, that it must be complete / exhaustive.
+  No partial derivation can ever be stored. Note also, that the result
+  is fixed in the type. This makes this structure rather clunky and tricky to use.
+  It may result in certain operations not being possible: If the result type
+  is not known at compile time.
+
+  - `.eps v h_v h_w`
+
+    - from the variable v we go to ε. Requires a proof that the
+        production is in the grammar.
+
+   - `.alpha v h_v h_w`
+
+    - from the variable v we go to a symbol that comprises w. Requires a proof that the
+        production is in the grammar.
+
+   - `.step v v' h_v h_w`
+
+    - Step constructor. Is a recursive call of the constructor.
+
+    - Requires a .cons production rule to have been applied.
+
+    - v' is generated by said .cons rule.
+
+    - w must have the shape `a :: w'`
+
+    - Finally, provide a RegularDerivation from v' to w'.
+-/
 inductive RegularDerivation (G: RegularGrammar α nt): (v: G.V) → (w: Word G.Z) → Type
 | eps (v: _) (h_v: .eps v ∈ G.productions) (h_w: w = ε):
   G.RegularDerivation v w
@@ -235,7 +302,7 @@ mutual
         exact h_w.symm
 
       . apply RegularDerivation.fromDerivation
-        exact derivation.cancelLeft h_u.symm h_w.symm
+        exact Grammar.Derivation.cancelLeft derivation h_u.symm h_w.symm
         rfl
   termination_by (derivation.len, 1)
   decreasing_by
